src/verification/kubernetes_model/simplereplicaset_init.v
@@ -1,11 +1,10 @@
-From New.proof Require Export context fmt.
+From New.proof Require Export fmt.
 From verification Require Export prelude.
 From verification.k8s_io.api.apps Require Export v1_init.
 From verification.k8s_io.api.core Require Export v1_init.
 From verification.k8s_io.apimachinery.pkg.api Require Export errors_init.
 From verification.k8s_io.apimachinery.pkg.apis.meta Require Export v1_init.
 From verification.k8s_io.apimachinery.pkg Require Export labels_init.
-From verification.k8s_io.client_go.tools Require Export cache_init.
 From verification.k8s_io.kubernetes.pkg Require Export controller_init.
 From verification.kubernetes_model Require Export simpleapiserver_init.
 Require Export New.generatedproof.kubernetes_model.simplereplicaset.
