src/verification/simplereplicaset.v
@@ -1,0 +1,30 @@
+From verification Require Import prelude empty_ffi simpleapiserver.
+From verification.kubernetes_model Require Export simplereplicaset_init.
+
+Section proof.
+Context `{!mapG Σ KKey.t KObject.t}.
+Context `{!mapG Σ KKey.t (gset KKey.t)}.
+Context `{!auth_setG Σ KKey.t}.
+Context `{hG: !heapGS Σ} {go_ctx: GoContext}.
+
+Lemma wp_syncReplicaSet (namespace name: go_string) γ_state γ_children γ_fresh_keys rs_key rs s (n: w32):
+  {{{ is_pkg_init simplereplicaset ∗
+      is_kubernetes_state γ_state γ_children γ_fresh_keys ∗
+      ⌜ rs_key = mk_replicaset_key namespace name ⌝ ∗
+      rs_key [[ γ_state ]]↦ KObject.ReplicaSet rs ∗
+      rs_key [[ γ_children ]]↦ s ∗
+      rs.(v1.ReplicaSet.Spec').(v1.ReplicaSetSpec.Replicas') ↦ n
+  }}}
+  @! simplereplicaset.syncReplicaSet #namespace #name
+  {{{ (err : error.t) s', RET #err;
+      rs_key [[ γ_children ]]↦ s' ∗
+      if decide (err = interface.nil) then
+        ⌜ size s' = sint.nat n ⌝
+      else
+        ⌜ Z.abs (Z.of_nat (size s') - sint.Z n) <
+          Z.abs (Z.of_nat (size s) - sint.Z n) ⌝
+  }}}.
+Proof. Admitted.
+
+
+End proof.
